Two principal properties over denotations: expansion law and monotonic ACI+id properties Cleaned up some proofs Corrected bad assumptions in CC theorems

Denotational.thy
@@ -5,6 +5,7 @@ imports
 
 begin
 
+(* Denotational interpretation of TESL *)
 fun TESL_interpretation_primitive
     :: "TESL_atomic \<Rightarrow> run set" ("\<lbrakk> _ \<rbrakk>\<^sub>T\<^sub>E\<^sub>S\<^sub>L") where
     "\<lbrakk> K sporadic \<tau> \<rbrakk>\<^sub>T\<^sub>E\<^sub>S\<^sub>L =
@@ -26,6 +27,7 @@ fun TESL_interpretation_primitive
                  )
         }"
 
+(* Denotational interpretation of TESL bounded by index *)
 fun TESL_interpretation_primitive_bounded
     :: "TESL_atomic \<Rightarrow> nat \<Rightarrow> run set" ("\<lbrakk> _ @\<le> _ \<rbrakk>\<^sub>T\<^sub>E\<^sub>S\<^sub>L") where
     "\<lbrakk> K sporadic \<tau> @\<le> b \<rbrakk>\<^sub>T\<^sub>E\<^sub>S\<^sub>L =
@@ -60,7 +62,8 @@ begin
 instance sorry
 end
 
-lemma "\<lbrakk> \<phi> \<rbrakk>\<^sub>T\<^sub>E\<^sub>S\<^sub>L = fst (gfp (\<lambda>(R, n). (R \<inter> \<lbrakk> \<phi> @\<le> n \<rbrakk>\<^sub>T\<^sub>E\<^sub>S\<^sub>L, n + 1)))"
+theorem TESL_interp_bnd_fixpoint:
+  shows "\<lbrakk> \<phi> \<rbrakk>\<^sub>T\<^sub>E\<^sub>S\<^sub>L = fst (gfp (\<lambda>(R, n). (R \<inter> \<lbrakk> \<phi> @\<le> n \<rbrakk>\<^sub>T\<^sub>E\<^sub>S\<^sub>L, n + 1)))"
 sorry
 
 (*
@@ -77,44 +80,211 @@ fun TESL_interpretation :: "TESL_formula \<Rightarrow> run set" ("\<lbrakk>\<lbr
     "\<lbrakk>\<lbrakk> [] \<rbrakk>\<rbrakk>\<^sub>T\<^sub>E\<^sub>S\<^sub>L = { _. True }"
   | "\<lbrakk>\<lbrakk> \<phi> # \<Phi> \<rbrakk>\<rbrakk>\<^sub>T\<^sub>E\<^sub>S\<^sub>L = \<lbrakk> \<phi> \<rbrakk>\<^sub>T\<^sub>E\<^sub>S\<^sub>L \<inter> \<lbrakk>\<lbrakk> \<Phi> \<rbrakk>\<rbrakk>\<^sub>T\<^sub>E\<^sub>S\<^sub>L"
 
-lemma symrun_refinement:
+(**) section \<open>Expansion law\<close> (**)
+text \<open>Similar to the expansion laws of lattices\<close>
+
+theorem TESL_interp_expansion:
+  shows "\<lbrakk>\<lbrakk> \<Phi>\<^sub>1 @ \<Phi>\<^sub>2 \<rbrakk>\<rbrakk>\<^sub>T\<^sub>E\<^sub>S\<^sub>L = \<lbrakk>\<lbrakk> \<Phi>\<^sub>1 \<rbrakk>\<rbrakk>\<^sub>T\<^sub>E\<^sub>S\<^sub>L \<inter> \<lbrakk>\<lbrakk> \<Phi>\<^sub>2 \<rbrakk>\<rbrakk>\<^sub>T\<^sub>E\<^sub>S\<^sub>L"
+sorry
+
+(**) section \<open>Equational laws for TESL formulae denotationally interpreted\<close> (**)
+(***) subsection \<open>General laws\<close> (***)
+
+lemma TESL_interp_assoc:
+  shows "\<lbrakk>\<lbrakk> (\<Phi>\<^sub>1 @ \<Phi>\<^sub>2) @ \<Phi>\<^sub>3 \<rbrakk>\<rbrakk>\<^sub>T\<^sub>E\<^sub>S\<^sub>L = \<lbrakk>\<lbrakk> \<Phi>\<^sub>1 @ (\<Phi>\<^sub>2 @ \<Phi>\<^sub>3) \<rbrakk>\<rbrakk>\<^sub>T\<^sub>E\<^sub>S\<^sub>L"
+  by auto
+
+lemma TESL_interp_commute:
+  shows "\<lbrakk>\<lbrakk> \<Phi>\<^sub>1 @ \<Phi>\<^sub>2 \<rbrakk>\<rbrakk>\<^sub>T\<^sub>E\<^sub>S\<^sub>L = \<lbrakk>\<lbrakk> \<Phi>\<^sub>2 @ \<Phi>\<^sub>1 \<rbrakk>\<rbrakk>\<^sub>T\<^sub>E\<^sub>S\<^sub>L"
+  by (simp add: TESL_interp_expansion inf_sup_aci(1))
+
+lemma TESL_interp_left_commute:
+  shows "\<lbrakk>\<lbrakk> \<Phi>\<^sub>1 @ (\<Phi>\<^sub>2 @ \<Phi>\<^sub>3) \<rbrakk>\<rbrakk>\<^sub>T\<^sub>E\<^sub>S\<^sub>L = \<lbrakk>\<lbrakk> \<Phi>\<^sub>2 @ (\<Phi>\<^sub>1 @ \<Phi>\<^sub>3) \<rbrakk>\<rbrakk>\<^sub>T\<^sub>E\<^sub>S\<^sub>L"
+  using TESL_interp_expansion by auto
+
+lemma TESL_interp_idem:
+  shows "\<lbrakk>\<lbrakk> \<Phi> @ \<Phi> \<rbrakk>\<rbrakk>\<^sub>T\<^sub>E\<^sub>S\<^sub>L = \<lbrakk>\<lbrakk> \<Phi> \<rbrakk>\<rbrakk>\<^sub>T\<^sub>E\<^sub>S\<^sub>L"
+  using TESL_interp_expansion by auto
+
+lemma TESL_interp_left_idem:
+  shows "\<lbrakk>\<lbrakk> \<Phi>\<^sub>1 @ (\<Phi>\<^sub>1 @ \<Phi>\<^sub>2) \<rbrakk>\<rbrakk>\<^sub>T\<^sub>E\<^sub>S\<^sub>L = \<lbrakk>\<lbrakk> \<Phi>\<^sub>1 @ \<Phi>\<^sub>2 \<rbrakk>\<rbrakk>\<^sub>T\<^sub>E\<^sub>S\<^sub>L"
+  using TESL_interp_expansion by auto
+
+lemma TESL_interp_right_idem:
+  shows "\<lbrakk>\<lbrakk> (\<Phi>\<^sub>1 @ \<Phi>\<^sub>2) @ \<Phi>\<^sub>2 \<rbrakk>\<rbrakk>\<^sub>T\<^sub>E\<^sub>S\<^sub>L = \<lbrakk>\<lbrakk> \<Phi>\<^sub>1 @ \<Phi>\<^sub>2 \<rbrakk>\<rbrakk>\<^sub>T\<^sub>E\<^sub>S\<^sub>L"
+  using TESL_interp_expansion by auto
+
+lemmas TESL_interp_aci = TESL_interp_commute TESL_interp_assoc TESL_interp_left_commute TESL_interp_left_idem
+
+(* Identity element *)
+lemma tesl_intersect_id_left [simp]: "\<lbrakk>\<lbrakk> [] @ \<Phi> \<rbrakk>\<rbrakk>\<^sub>T\<^sub>E\<^sub>S\<^sub>L = \<lbrakk>\<lbrakk> \<Phi> \<rbrakk>\<rbrakk>\<^sub>T\<^sub>E\<^sub>S\<^sub>L"
+by simp
+
+lemma tesl_intersect_id_right [simp]: "\<lbrakk>\<lbrakk> \<Phi> @ [] \<rbrakk>\<rbrakk>\<^sub>T\<^sub>E\<^sub>S\<^sub>L = \<lbrakk>\<lbrakk> \<Phi> \<rbrakk>\<rbrakk>\<^sub>T\<^sub>E\<^sub>S\<^sub>L"
+by simp
+
+find_theorems "_ \<inter> _ = _"
+section \<open>Decreasing interpretation of TESL formulae\<close>
+
+lemma TESL_sem_decreases_head:
   "\<lbrakk>\<lbrakk> \<Phi> \<rbrakk>\<rbrakk>\<^sub>T\<^sub>E\<^sub>S\<^sub>L \<supseteq> \<lbrakk>\<lbrakk> \<phi> # \<Phi> \<rbrakk>\<rbrakk>\<^sub>T\<^sub>E\<^sub>S\<^sub>L"
 by simp
 
-lemma symrun_refinement':
-  assumes inc: "set \<Phi> \<subseteq> set \<Phi>'"
-  shows "\<lbrakk>\<lbrakk> \<Phi> \<rbrakk>\<rbrakk>\<^sub>T\<^sub>E\<^sub>S\<^sub>L \<supseteq> \<lbrakk>\<lbrakk> \<Phi>' \<rbrakk>\<rbrakk>\<^sub>T\<^sub>E\<^sub>S\<^sub>L"
-sorry
+lemma TESL_sem_decreases_tail:
+  "\<lbrakk>\<lbrakk> \<Phi> \<rbrakk>\<rbrakk>\<^sub>T\<^sub>E\<^sub>S\<^sub>L \<supseteq> \<lbrakk>\<lbrakk> \<Phi> @ [\<phi>] \<rbrakk>\<rbrakk>\<^sub>T\<^sub>E\<^sub>S\<^sub>L"
+  by (simp add: TESL_interp_expansion)
 
-text \<open> Every TESL formula denotes a satisfying run \<close>
-(* Missing hypothesis that the linear system made of tag relations is consistent *)
-lemma existence:
-  shows "\<exists>\<rho>. \<rho> \<in> \<lbrakk>\<lbrakk> \<Phi> \<rbrakk>\<rbrakk>\<^sub>T\<^sub>E\<^sub>S\<^sub>L"
-oops
+
+(** Draft attempts of Burkhart *)
 (*
-proof (induction \<Phi>)
+lemma extension_monotone_generqalized1:
+  shows "\<lbrakk>\<lbrakk> \<Phi>' @ \<Phi> \<rbrakk>\<rbrakk>\<^sub>T\<^sub>E\<^sub>S\<^sub>L \<subseteq> \<lbrakk>\<lbrakk> \<Phi> \<rbrakk>\<rbrakk>\<^sub>T\<^sub>E\<^sub>S\<^sub>L"
+proof(induct "\<Phi>'")
+    case Nil
+    then show ?case by simp
+next
+    case (Cons a \<Phi>')
+    then show ?case by auto
+qed
+
+lemma extension_distr:
+  shows "\<lbrakk>\<lbrakk> \<Phi> @ \<Phi>' \<rbrakk>\<rbrakk>\<^sub>T\<^sub>E\<^sub>S\<^sub>L =  \<lbrakk>\<lbrakk> \<Phi> \<rbrakk>\<rbrakk>\<^sub>T\<^sub>E\<^sub>S\<^sub>L \<inter> \<lbrakk>\<lbrakk> \<Phi>' \<rbrakk>\<rbrakk>\<^sub>T\<^sub>E\<^sub>S\<^sub>L"
+proof(induct "\<Phi>")
   case Nil
   then show ?case by simp
 next
-  case (Cons \<phi> \<Phi>')
-  then show ?case
-    proof (induction \<phi>)
-      case (Sporadic K \<tau>)      
-      then show ?case sorry
-    next
-      case (Implies master slave)
-      then show ?case sorry
-    next
-      case (SporadicOn x1 x2 x3)
-      then show ?case sorry
-    next
-      case (TagRelation x1 x2 x3 x4)
-      then show ?case sorry
-    next
-      case (TimeDelayedBy x1 x2 x3 x4)
-      then show ?case sorry
-    qed
+  case (Cons a \<Phi>)
+  then show ?case by auto
 qed
+
+lemma set_append_mono: "set \<Phi> \<subseteq> set \<Phi>' \<Longrightarrow> \<exists> \<Phi>'' . set \<Phi>' =  set(\<Phi>'' @ \<Phi>)" 
+sorry
+
+lemma elim_remove1 : "x \<in> set S \<Longrightarrow> \<exists> T T'. remove1 x S = T @ T' \<and> S = T @ [x] @ T' "
+sorry
+
+
+find_theorems "_ \<in> _" "remove1"
+lemma "set \<Phi> =  set \<Phi>' \<Longrightarrow> set (remove1 n \<Phi>) =  set (remove1 n \<Phi>')"
+sorry
+
+lemma XXX: "\<lbrakk>\<lbrakk> \<Phi> \<rbrakk>\<rbrakk>\<^sub>T\<^sub>E\<^sub>S\<^sub>L = \<lbrakk>\<lbrakk> remdups \<Phi> \<rbrakk>\<rbrakk>\<^sub>T\<^sub>E\<^sub>S\<^sub>L"
+sorry
+
+lemma  "length \<Phi> \<le> n \<Longrightarrow> length \<Phi>' \<le> n \<Longrightarrow> set \<Phi> =  set \<Phi>'\<Longrightarrow> \<lbrakk>\<lbrakk> \<Phi> \<rbrakk>\<rbrakk>\<^sub>T\<^sub>E\<^sub>S\<^sub>L =  \<lbrakk>\<lbrakk> \<Phi>' \<rbrakk>\<rbrakk>\<^sub>T\<^sub>E\<^sub>S\<^sub>L" 
+proof(induct n arbitrary: \<Phi> \<Phi>') print_cases
+  case 0
+  then show ?case by simp
+next
+  case (Suc n)
+     have * : "\<And>n \<Phi> . length \<Phi> = Suc n \<Longrightarrow> \<exists> n. n \<in> set \<Phi>"
+              using length_Suc_conv by fastforce
+     have **: "length \<Phi> = 0 \<Longrightarrow> \<Phi> = []"
+              by simp
+  show ?case 
+     apply(insert Suc.hyps Suc.prems)
+     proof(cases "length \<Phi> \<le> length \<Phi>'")
+       case True
+       then show ?thesis
+            proof(cases "length \<Phi>' = Suc n")
+              case True
+              then show ?thesis
+                 apply(insert *[OF `length \<Phi>' = Suc n`], elim exE, simp)
+                 proof - 
+                    fix m
+                    assume 1: "m \<in> set \<Phi>'" and 2: " length \<Phi>' = Suc n"
+                    have *** : "m \<in> set \<Phi>"  by (simp add: Suc.prems(3) \<open>m \<in> set \<Phi>'\<close>)
+                    show "\<lbrakk>\<lbrakk> \<Phi> \<rbrakk>\<rbrakk>\<^sub>T\<^sub>E\<^sub>S\<^sub>L = \<lbrakk>\<lbrakk> \<Phi>' \<rbrakk>\<rbrakk>\<^sub>T\<^sub>E\<^sub>S\<^sub>L"                       
+                      apply(insert 1, drule elim_remove1, insert ***, drule elim_remove1, clarsimp)
+                      apply(simp add: extension_distr)
+find_theorems (140)"_ \<inter> _ = _ " name:"Set"
+                      apply(subst Set.Int_assoc[symmetric])
+                      apply(subst Set.Int_commute)
+                      apply(subst Set.Int_assoc[symmetric])
+                      apply(subst (3) Set.Int_commute)
+                      apply(subst Set.Int_assoc)
+                      apply(subst Set.Int_assoc)
+                      apply(subst extension_distr[symmetric])
+                      apply(subst extension_distr[symmetric])
+                      apply(subst Suc.hyps)
+                      prefer 4 apply(rule refl)
+                      using Suc.prems(1) apply auto[1]
+                      using True apply auto[1]
+                      apply(insert Suc.prems)
+(* sledgehammer *)
+ sorry
+            next
+              case False
+              then show ?thesis sorry
+            qed
+ sorry
+     next
+       case False
+       then show ?thesis sorry
+     qed 
+sledgehammer
+ sorry
+qed
+
+lemma  "set \<Phi> =  set \<Phi>' \<Longrightarrow> \<lbrakk>\<lbrakk> \<Phi> \<rbrakk>\<rbrakk>\<^sub>T\<^sub>E\<^sub>S\<^sub>L =  \<lbrakk>\<lbrakk> \<Phi>' \<rbrakk>\<rbrakk>\<^sub>T\<^sub>E\<^sub>S\<^sub>L" 
+find_theorems (450) "set _ = set _"
+sorry
+
+lemma **:
+  assumes "set \<Phi> \<subseteq> set \<Phi>'"
+  shows "\<lbrakk>\<lbrakk> \<Phi>' \<rbrakk>\<rbrakk>\<^sub>T\<^sub>E\<^sub>S\<^sub>L \<subseteq> \<lbrakk>\<lbrakk> \<Phi> \<rbrakk>\<rbrakk>\<^sub>T\<^sub>E\<^sub>S\<^sub>L"
+apply(insert assms[THEN set_append_mono], clarsimp)
+sorry
 *)
+
+theorem TESL_interp_decreases_setinc:
+  assumes incl: "set \<Phi> \<subseteq> set \<Phi>'"
+  shows "\<lbrakk>\<lbrakk> \<Phi> \<rbrakk>\<rbrakk>\<^sub>T\<^sub>E\<^sub>S\<^sub>L \<supseteq> \<lbrakk>\<lbrakk> \<Phi>' \<rbrakk>\<rbrakk>\<^sub>T\<^sub>E\<^sub>S\<^sub>L"
+sorry
+
+lemma TESL_interp_decreases_add_head:
+  assumes incl: "set \<Phi> \<subseteq> set \<Phi>'"
+  shows "\<lbrakk>\<lbrakk> \<phi> # \<Phi> \<rbrakk>\<rbrakk>\<^sub>T\<^sub>E\<^sub>S\<^sub>L \<supseteq> \<lbrakk>\<lbrakk> \<phi> # \<Phi>' \<rbrakk>\<rbrakk>\<^sub>T\<^sub>E\<^sub>S\<^sub>L"
+  using TESL_interp_decreases_setinc incl by auto
+
+lemma TESL_interp_decreases_add_tail:
+  assumes incl: "set \<Phi> \<subseteq> set \<Phi>'"
+  shows "\<lbrakk>\<lbrakk> \<Phi> @ [\<phi>] \<rbrakk>\<rbrakk>\<^sub>T\<^sub>E\<^sub>S\<^sub>L \<supseteq> \<lbrakk>\<lbrakk> \<Phi>' @ [\<phi>] \<rbrakk>\<rbrakk>\<^sub>T\<^sub>E\<^sub>S\<^sub>L"
+  by (metis TESL_interp_commute TESL_interp_decreases_add_head append_Cons append_Nil incl)
+
+lemma TESL_interp_absorb1:
+  assumes incl: "set \<Phi>\<^sub>1 \<subseteq> set \<Phi>\<^sub>2"
+  shows "\<lbrakk>\<lbrakk> \<Phi>\<^sub>1 @ \<Phi>\<^sub>2 \<rbrakk>\<rbrakk>\<^sub>T\<^sub>E\<^sub>S\<^sub>L = \<lbrakk>\<lbrakk> \<Phi>\<^sub>2 \<rbrakk>\<rbrakk>\<^sub>T\<^sub>E\<^sub>S\<^sub>L"
+  by (simp add: Int_absorb1 TESL_interp_decreases_setinc TESL_interp_expansion incl)
+
+lemma TESL_interp_absorb2:
+  assumes incl: "set \<Phi>\<^sub>2 \<subseteq> set \<Phi>\<^sub>1"
+  shows "\<lbrakk>\<lbrakk> \<Phi>\<^sub>1 @ \<Phi>\<^sub>2 \<rbrakk>\<rbrakk>\<^sub>T\<^sub>E\<^sub>S\<^sub>L = \<lbrakk>\<lbrakk> \<Phi>\<^sub>1 \<rbrakk>\<rbrakk>\<^sub>T\<^sub>E\<^sub>S\<^sub>L"
+  using TESL_interp_absorb1 TESL_interp_commute incl by blast
+
+(***) subsection \<open>Case of filtering out sporadic atoms\<close> (***)
+
+lemma NoSporadic_stable [simp]:
+  shows "\<lbrakk>\<lbrakk> \<Phi> \<rbrakk>\<rbrakk>\<^sub>T\<^sub>E\<^sub>S\<^sub>L \<subseteq> \<lbrakk>\<lbrakk> NoSporadic \<Phi> \<rbrakk>\<rbrakk>\<^sub>T\<^sub>E\<^sub>S\<^sub>L"
+  by (meson filter_is_subset TESL_interp_decreases_setinc)
+
+lemma NoSporadic_idem [simp]:
+  shows "\<lbrakk>\<lbrakk> \<Phi> \<rbrakk>\<rbrakk>\<^sub>T\<^sub>E\<^sub>S\<^sub>L \<inter> \<lbrakk>\<lbrakk> NoSporadic \<Phi> \<rbrakk>\<rbrakk>\<^sub>T\<^sub>E\<^sub>S\<^sub>L = \<lbrakk>\<lbrakk> \<Phi> \<rbrakk>\<rbrakk>\<^sub>T\<^sub>E\<^sub>S\<^sub>L"
+  by (meson Int_absorb2 filter_is_subset TESL_interp_decreases_setinc)
+
+lemma NoSporadic_setinc:
+  shows "set (NoSporadic \<Phi>) \<subseteq> set \<Phi>"
+by auto
+
+(**) section \<open>Run existence for TESL arithmetic-consistent formulae\<close> (**)
+fun tagrel_consistent :: "TESL_formula \<Rightarrow> bool" where
+  "tagrel_consistent \<Phi> = undefined"
+
+lemma existence:
+  (* Assumption that the linear system made of tag relations is consistent *)
+  assumes "tagrel_consistent \<Phi>"
+  shows "\<exists>\<rho>. \<rho> \<in> \<lbrakk>\<lbrakk> \<Phi> \<rbrakk>\<rbrakk>\<^sub>T\<^sub>E\<^sub>S\<^sub>L"
+oops
+(* proof (induction \<Phi>) *)
 
 end
