Run.thy
@@ -44,19 +44,10 @@ fun symbolic_run_interpretation :: "constr list \<Rightarrow> run set" ("\<lbrak
     "\<lbrakk>\<lbrakk> [] \<rbrakk>\<rbrakk>\<^sub>s\<^sub>y\<^sub>m\<^sub>r\<^sub>u\<^sub>n = { _. True }"
   | "\<lbrakk>\<lbrakk> \<gamma> # \<Gamma> \<rbrakk>\<rbrakk>\<^sub>s\<^sub>y\<^sub>m\<^sub>r\<^sub>u\<^sub>n = \<lbrakk> \<gamma> \<rbrakk>\<^sub>s\<^sub>y\<^sub>m\<^sub>r\<^sub>u\<^sub>n \<inter> \<lbrakk>\<lbrakk> \<Gamma> \<rbrakk>\<rbrakk>\<^sub>s\<^sub>y\<^sub>m\<^sub>r\<^sub>u\<^sub>n"
 
-lemma symrun_refinement:
-  "\<lbrakk>\<lbrakk> \<Gamma> \<rbrakk>\<rbrakk>\<^sub>s\<^sub>y\<^sub>m\<^sub>r\<^sub>u\<^sub>n \<supseteq> \<lbrakk>\<lbrakk> \<gamma> # \<Gamma> \<rbrakk>\<rbrakk>\<^sub>s\<^sub>y\<^sub>m\<^sub>r\<^sub>u\<^sub>n"
-by simp
-
-lemma symrun_refinement':
-  assumes inc: "set \<Gamma> \<subseteq> set \<Gamma>'"
-  shows "\<lbrakk>\<lbrakk> \<Gamma> \<rbrakk>\<rbrakk>\<^sub>s\<^sub>y\<^sub>m\<^sub>r\<^sub>u\<^sub>n \<supseteq> \<lbrakk>\<lbrakk> \<Gamma>' \<rbrakk>\<rbrakk>\<^sub>s\<^sub>y\<^sub>m\<^sub>r\<^sub>u\<^sub>n"
-sorry
-
 definition consistent_run :: "constr list \<Rightarrow> bool" where 
   "consistent_run \<Gamma> \<equiv> \<exists>\<rho>. \<rho> \<in> \<lbrakk>\<lbrakk> \<Gamma> \<rbrakk>\<rbrakk>\<^sub>s\<^sub>y\<^sub>m\<^sub>r\<^sub>u\<^sub>n"
 
-text \<open> Defining a method for witness construction \<close>
+(**) section \<open>Defining a method for witness construction\<close> (**)
 
 (* Initial states *)
 abbreviation initial_run :: "run" ("\<rho>\<^sub>\<odot>") where
@@ -93,5 +84,123 @@ lemma witness_consistency:
 lemma witness_consistency':
   "consistent_run \<Gamma> \<Longrightarrow> \<langle>\<langle> \<Gamma> \<rangle>\<rangle> \<in> \<lbrakk>\<lbrakk> \<Gamma> \<rbrakk>\<rbrakk>\<^sub>s\<^sub>y\<^sub>m\<^sub>r\<^sub>u\<^sub>n"
   oops (* Not sure the idea is true *)
+
+(**) section \<open>Rules and properties of consistence\<close> (**)
+
+lemma context_consistency_preservationI:
+  "consistent_run (\<gamma> # \<Gamma>) \<Longrightarrow> consistent_run \<Gamma>"
+using consistent_run_def by auto
+
+(* This is very restrictive *)
+inductive context_independency :: "constr \<Rightarrow> constr list \<Rightarrow> bool" ("_ \<bowtie> _") where
+  NotTicks_independency:
+  "K \<Up> n \<notin> set \<Gamma> \<Longrightarrow> K \<not>\<Up> n \<bowtie> \<Gamma>"
+| Ticks_independency:
+  "K \<not>\<Up> n \<notin> set \<Gamma> \<Longrightarrow> K \<Up> n \<bowtie> \<Gamma>"
+| Timestamp_independency:
+  "(\<nexists>\<tau>'. \<tau>' = \<tau> \<and> K \<Down> n @ \<tau> \<in> set \<Gamma>) \<Longrightarrow> K \<Down> n @ \<tau> \<bowtie> \<Gamma>"
+
+thm context_independency.induct
+
+lemma context_consistency_preservationE:
+  assumes consist: "consistent_run \<Gamma>"
+  and     indepen: "\<gamma> \<bowtie> \<Gamma>"
+  shows "consistent_run (\<gamma> # \<Gamma>)"
+apply (insert consist indepen)
+apply (erule context_independency.cases)
+apply auto
+proof -
+  show "\<And>K n. consistent_run \<Gamma> \<Longrightarrow>
+           \<gamma> = K \<not>\<Up> n \<Longrightarrow> K \<Up> n \<notin> set \<Gamma> \<Longrightarrow>
+           consistent_run (K \<not>\<Up> n # \<Gamma>)"
+    sorry
+  show "\<And>K n. consistent_run \<Gamma> \<Longrightarrow>
+           \<gamma> = K \<Up> n \<Longrightarrow> K \<not>\<Up> n \<notin> set \<Gamma> \<Longrightarrow>
+           consistent_run (K \<Up> n # \<Gamma>)"
+    sorry
+  show "\<And>\<tau> K n.
+       consistent_run \<Gamma> \<Longrightarrow>
+       \<gamma> = K \<Down> n @ \<tau> \<Longrightarrow>
+       K \<Down> n @ \<tau> \<notin> set \<Gamma> \<Longrightarrow> consistent_run (K \<Down> n @ \<tau> # \<Gamma>)"
+    sorry
+qed
+
+(**) section \<open>Expansion law\<close> (**)
+text \<open>Similar to the expansion laws of lattices\<close>
+
+theorem symrun_interp_expansion:
+  shows "\<lbrakk>\<lbrakk> \<Gamma>\<^sub>1 @ \<Gamma>\<^sub>2 \<rbrakk>\<rbrakk>\<^sub>s\<^sub>y\<^sub>m\<^sub>r\<^sub>u\<^sub>n = \<lbrakk>\<lbrakk> \<Gamma>\<^sub>1 \<rbrakk>\<rbrakk>\<^sub>s\<^sub>y\<^sub>m\<^sub>r\<^sub>u\<^sub>n \<inter> \<lbrakk>\<lbrakk> \<Gamma>\<^sub>2 \<rbrakk>\<rbrakk>\<^sub>s\<^sub>y\<^sub>m\<^sub>r\<^sub>u\<^sub>n"
+sorry
+
+(**) section \<open>A few equational laws\<close> (**)
+
+lemma symrun_interp_assoc:
+  shows "\<lbrakk>\<lbrakk> (\<Gamma>\<^sub>1 @ \<Gamma>\<^sub>2) @ \<Gamma>\<^sub>3 \<rbrakk>\<rbrakk>\<^sub>s\<^sub>y\<^sub>m\<^sub>r\<^sub>u\<^sub>n = \<lbrakk>\<lbrakk> \<Gamma>\<^sub>1 @ (\<Gamma>\<^sub>2 @ \<Gamma>\<^sub>3) \<rbrakk>\<rbrakk>\<^sub>s\<^sub>y\<^sub>m\<^sub>r\<^sub>u\<^sub>n"
+  by auto
+
+lemma symrun_interp_commute:
+  shows "\<lbrakk>\<lbrakk> \<Gamma>\<^sub>1 @ \<Gamma>\<^sub>2 \<rbrakk>\<rbrakk>\<^sub>s\<^sub>y\<^sub>m\<^sub>r\<^sub>u\<^sub>n = \<lbrakk>\<lbrakk> \<Gamma>\<^sub>2 @ \<Gamma>\<^sub>1 \<rbrakk>\<rbrakk>\<^sub>s\<^sub>y\<^sub>m\<^sub>r\<^sub>u\<^sub>n"
+  by (simp add: symrun_interp_expansion inf_sup_aci(1))
+
+lemma symrun_interp_left_commute:
+  shows "\<lbrakk>\<lbrakk> \<Gamma>\<^sub>1 @ (\<Gamma>\<^sub>2 @ \<Gamma>\<^sub>3) \<rbrakk>\<rbrakk>\<^sub>s\<^sub>y\<^sub>m\<^sub>r\<^sub>u\<^sub>n = \<lbrakk>\<lbrakk> \<Gamma>\<^sub>2 @ (\<Gamma>\<^sub>1 @ \<Gamma>\<^sub>3) \<rbrakk>\<rbrakk>\<^sub>s\<^sub>y\<^sub>m\<^sub>r\<^sub>u\<^sub>n"
+  using symrun_interp_expansion by auto
+
+lemma symrun_interp_idem:
+  shows "\<lbrakk>\<lbrakk> \<Gamma> @ \<Gamma> \<rbrakk>\<rbrakk>\<^sub>s\<^sub>y\<^sub>m\<^sub>r\<^sub>u\<^sub>n = \<lbrakk>\<lbrakk> \<Gamma> \<rbrakk>\<rbrakk>\<^sub>s\<^sub>y\<^sub>m\<^sub>r\<^sub>u\<^sub>n"
+  using symrun_interp_expansion by auto
+
+lemma symrun_interp_left_idem:
+  shows "\<lbrakk>\<lbrakk> \<Gamma>\<^sub>1 @ (\<Gamma>\<^sub>1 @ \<Gamma>\<^sub>2) \<rbrakk>\<rbrakk>\<^sub>s\<^sub>y\<^sub>m\<^sub>r\<^sub>u\<^sub>n = \<lbrakk>\<lbrakk> \<Gamma>\<^sub>1 @ \<Gamma>\<^sub>2 \<rbrakk>\<rbrakk>\<^sub>s\<^sub>y\<^sub>m\<^sub>r\<^sub>u\<^sub>n"
+  using symrun_interp_expansion by auto
+
+lemma symrun_interp_right_idem:
+  shows "\<lbrakk>\<lbrakk> (\<Gamma>\<^sub>1 @ \<Gamma>\<^sub>2) @ \<Gamma>\<^sub>2 \<rbrakk>\<rbrakk>\<^sub>s\<^sub>y\<^sub>m\<^sub>r\<^sub>u\<^sub>n = \<lbrakk>\<lbrakk> \<Gamma>\<^sub>1 @ \<Gamma>\<^sub>2 \<rbrakk>\<rbrakk>\<^sub>s\<^sub>y\<^sub>m\<^sub>r\<^sub>u\<^sub>n"
+  using symrun_interp_expansion by auto
+
+lemmas symrun_interp_aci = symrun_interp_commute symrun_interp_assoc symrun_interp_left_commute symrun_interp_left_idem
+
+lemma tesl_intersect_id_left [simp]: "\<lbrakk>\<lbrakk> [] @ \<Gamma> \<rbrakk>\<rbrakk>\<^sub>s\<^sub>y\<^sub>m\<^sub>r\<^sub>u\<^sub>n = \<lbrakk>\<lbrakk> \<Gamma> \<rbrakk>\<rbrakk>\<^sub>s\<^sub>y\<^sub>m\<^sub>r\<^sub>u\<^sub>n"
+by simp
+
+lemma tesl_intersect_id_right [simp]: "\<lbrakk>\<lbrakk> \<Gamma> @ [] \<rbrakk>\<rbrakk>\<^sub>s\<^sub>y\<^sub>m\<^sub>r\<^sub>u\<^sub>n = \<lbrakk>\<lbrakk> \<Gamma> \<rbrakk>\<rbrakk>\<^sub>s\<^sub>y\<^sub>m\<^sub>r\<^sub>u\<^sub>n"
+by simp
+
+find_theorems "_ \<inter> _ = _"
+section \<open>Decreasing interpretation of TESL formulae\<close>
+
+lemma symrun_sem_decreases_head:
+  "\<lbrakk>\<lbrakk> \<Gamma> \<rbrakk>\<rbrakk>\<^sub>s\<^sub>y\<^sub>m\<^sub>r\<^sub>u\<^sub>n \<supseteq> \<lbrakk>\<lbrakk> \<phi> # \<Gamma> \<rbrakk>\<rbrakk>\<^sub>s\<^sub>y\<^sub>m\<^sub>r\<^sub>u\<^sub>n"
+by simp
+
+lemma symrun_sem_decreases_tail:
+  "\<lbrakk>\<lbrakk> \<Gamma> \<rbrakk>\<rbrakk>\<^sub>s\<^sub>y\<^sub>m\<^sub>r\<^sub>u\<^sub>n \<supseteq> \<lbrakk>\<lbrakk> \<Gamma> @ [\<phi>] \<rbrakk>\<rbrakk>\<^sub>s\<^sub>y\<^sub>m\<^sub>r\<^sub>u\<^sub>n"
+  by (simp add: symrun_interp_expansion)
+
+theorem symrun_interp_decreases_setinc:
+  assumes incl: "set \<Gamma> \<subseteq> set \<Gamma>'"
+  shows "\<lbrakk>\<lbrakk> \<Gamma> \<rbrakk>\<rbrakk>\<^sub>s\<^sub>y\<^sub>m\<^sub>r\<^sub>u\<^sub>n \<supseteq> \<lbrakk>\<lbrakk> \<Gamma>' \<rbrakk>\<rbrakk>\<^sub>s\<^sub>y\<^sub>m\<^sub>r\<^sub>u\<^sub>n"
+sorry
+
+lemma symrun_interp_decreases_add_head:
+  assumes incl: "set \<Gamma> \<subseteq> set \<Gamma>'"
+  shows "\<lbrakk>\<lbrakk> \<phi> # \<Gamma> \<rbrakk>\<rbrakk>\<^sub>s\<^sub>y\<^sub>m\<^sub>r\<^sub>u\<^sub>n \<supseteq> \<lbrakk>\<lbrakk> \<phi> # \<Gamma>' \<rbrakk>\<rbrakk>\<^sub>s\<^sub>y\<^sub>m\<^sub>r\<^sub>u\<^sub>n"
+  using symrun_interp_decreases_setinc incl by auto
+
+lemma symrun_interp_decreases_add_tail:
+  assumes incl: "set \<Gamma> \<subseteq> set \<Gamma>'"
+  shows "\<lbrakk>\<lbrakk> \<Gamma> @ [\<phi>] \<rbrakk>\<rbrakk>\<^sub>s\<^sub>y\<^sub>m\<^sub>r\<^sub>u\<^sub>n \<supseteq> \<lbrakk>\<lbrakk> \<Gamma>' @ [\<phi>] \<rbrakk>\<rbrakk>\<^sub>s\<^sub>y\<^sub>m\<^sub>r\<^sub>u\<^sub>n"
+  by (metis symrun_interp_commute symrun_interp_decreases_add_head append_Cons append_Nil incl)
+
+lemma symrun_interp_absorb1:
+  assumes incl: "set \<Gamma>\<^sub>1 \<subseteq> set \<Gamma>\<^sub>2"
+  shows "\<lbrakk>\<lbrakk> \<Gamma>\<^sub>1 @ \<Gamma>\<^sub>2 \<rbrakk>\<rbrakk>\<^sub>s\<^sub>y\<^sub>m\<^sub>r\<^sub>u\<^sub>n = \<lbrakk>\<lbrakk> \<Gamma>\<^sub>2 \<rbrakk>\<rbrakk>\<^sub>s\<^sub>y\<^sub>m\<^sub>r\<^sub>u\<^sub>n"
+  by (simp add: Int_absorb1 symrun_interp_decreases_setinc symrun_interp_expansion incl)
+
+lemma symrun_interp_absorb2:
+  assumes incl: "set \<Gamma>\<^sub>2 \<subseteq> set \<Gamma>\<^sub>1"
+  shows "\<lbrakk>\<lbrakk> \<Gamma>\<^sub>1 @ \<Gamma>\<^sub>2 \<rbrakk>\<rbrakk>\<^sub>s\<^sub>y\<^sub>m\<^sub>r\<^sub>u\<^sub>n = \<lbrakk>\<lbrakk> \<Gamma>\<^sub>1 \<rbrakk>\<rbrakk>\<^sub>s\<^sub>y\<^sub>m\<^sub>r\<^sub>u\<^sub>n"
+  using symrun_interp_absorb1 symrun_interp_commute incl by blast
+
 
 end
